examples/append.v
@@ -1,0 +1,86 @@
+From Stdlib Require Import List String ZArith.
+From shift_reset.lib Require sum.
+From shift_reset.core Require Import syntax syntax_notation coerce.
+From shift_reset.interpreter Require Import interpreter.
+From examples.lib Require Import list.
+Import ListNotations.
+
+Open Scope Z_scope.
+Open Scope string_scope.
+Open Scope term_scope.
+
+Definition range (s e : Z) :=
+  let fix go s l :=
+    match l with
+    | O => []
+    | S l' => s :: go (s + 1) l'
+    end
+  in
+  go s (Z.to_nat (e - s)).
+
+Example append_dcont_aux :=
+  <{ fun "xs" =>
+       let fix "go" "xs" :=
+         match "xs" with
+         | Inl _ => shift (fun "k" => "k")
+         | Inr "p" =>
+             let ("x", "xs'") := "p" in
+             let "r" := "go" "xs'" in
+             Inr ("x", "r")
+         end
+       in
+       reset "go" "xs" }>.
+
+Example append_dcont :=
+  <{ fun "args" =>
+       let ("xs", "ys") := "args" in
+       let "k" := append_dcont_aux "xs" in
+       "k" "ys" }>.
+
+Example append :=
+  <{ fix "go" "args" :=
+       let ("xs", "ys") := "args" in
+       match "xs" with
+       | Inl _ => "ys"
+       | Inr "p" =>
+           let ("x", "xs'") := "p" in
+           let "r" := "go" ("xs'", "ys") in
+           Inr ("x", "r")
+       end }>.
+
+Example append_curry_aux :=
+  <{ fix "go" "xs" "ys" :=
+       match "xs" with
+       | Inl _ => "ys"
+       | Inr "p" =>
+           let ("x", "xs'") := "p" in
+           let "k" := "go" "xs'" in
+           let "r" := "k" "ys" in
+           Inr ("x", "r")
+       end }>.
+
+Example append_curry :=
+  <{ fun "args" =>
+       let ("xs", "ys") := "args" in
+       let "k" := append_curry_aux "xs" in
+       "k" "ys" }>.
+
+Definition eval_append (candidate : val_term) (fuel : nat) (xs ys : list Z) :=
+  eval_term_to_int_list fuel <{ candidate ({int_list_to_val_term xs}, {int_list_to_val_term ys}) }>.
+
+Compute (eval_term 3 <{ append_dcont_aux {int_list_to_val_term []} }>).
+Compute (eval_term 4 <{ append_dcont_aux {int_list_to_val_term [1]} }>).
+Compute (eval_term 5 <{ append_dcont_aux {int_list_to_val_term [1; 2]} }>).
+
+Compute (eval_append append 2 [] [69]).
+Compute (eval_append append 3 [1] [69]).
+Compute (eval_append append 4 [1; 2] [69]).
+Compute (eval_append append_dcont 4 [] [69]).
+Compute (eval_append append_dcont 5 [1] [69]).
+Compute (eval_append append_dcont 6 [1; 2] [69]).
+Compute (eval_append append_curry 4 [] [69]).
+Compute (eval_append append_curry 5 [1] [69]).
+Compute (eval_append append_curry 6 [1; 2] [69]).
+Time Compute (sum.map (@List.length _) (eval_append append 12800 (range 0 12710) [])).
+Time Compute (sum.map (@List.length _) (eval_append append_dcont 12800 (range 0 12710) [])).
+Time Compute (sum.map (@List.length _) (eval_append append_curry 12800 (range 0 12710) [])).
