examples/fib_it.v
@@ -7,15 +7,24 @@ Open Scope Z_scope.
 Open Scope string_scope.
 Open Scope term_scope.
 
+Example fib_it :=
+  <{ fun _ =>
+       let fix "go" "args" :=
+         let ("a", "b") := "args" in
+         Inr ("a", fun _ => "go" ("b", "a" + "b"))
+       in
+       "go" (0, 1) }>.
+
 Example yield := <{ fun "v" => shift (fun "k" => Inr ("v", "k")) }>.
 
-Example fib_it :=
+Example fib_it_dcont :=
   <{ fun _ =>
        let fix "go" "args" :=
          let ("a", "b") := "args" in
          yield "a";
          "go" ("b", "a" + "b")
-       in reset "go" (0, 1) }>.
+       in
+       reset "go" (0, 1) }>.
 
 Example take :=
   <{ fix "go" "args" :=
@@ -31,7 +40,8 @@ Example take :=
              Inr ("v", "vs")
          end }>.
 
-Example eval_fib (fuel : nat) (n : Z) :=
-  eval_term_to_int_list fuel <{ take (n, fib_it) }>.
+Example eval_fib (candidate : val_term) (fuel : nat) (n : Z) :=
+  eval_term_to_int_list fuel <{ take (n, candidate) }>.
 
-Compute (eval_fib 100 50).
+Compute (eval_fib fib_it 100 50).
+Compute (eval_fib fib_it_dcont 100 50).
